\documentclass[a4paper,12pt]{article}

% Variables
\title{Calculating the sum of $n$ squares}

% Body
\begin{document}

% Insert title
\maketitle

The sum of squares of the first $n$ integers can be simplified with:
$$
1^2 + 2^2 + ... + n^2 = \frac{n^3}{3} + \frac{n^2}{2} + \frac{n}{6}
$$

We start from the simple cube of binomium:
$$
(k + 1)^3 = k^3 + 3k^2 + 3k + 1
$$

Moving the terms slightly we get:
$$
3k^2 + 3k + 1 = (k + 1)^3 - k^3
$$

Assigning $k = 1, 2, ... n - 1$ the formulas become:
$$
3\cdot1^2 + 3\cdot1 + 1 = 2^3 - 1^3
$$
$$
3\cdot2^2 + 3\cdot2 + 1 = 3^3 - 2^3
$$

$$
3(n - 1)^2 + 3(n - 1) + 1 = n^3 - (n - 1)^3
$$

Adding the three formulas and canceling:
$$
3[1^2 + 2^2 + ... + (n - 1)^2] + 3[1 + 2 + ... + (n - 1)] + (n - 1) = n^3 - 1^3
$$

The second sum on the left is a succession the sum of which is $\frac{n(n-1)}{2}$.
$$
3[1^2 + 2^2 + ... + (n - 1)^2] + \frac{3}{2}n(n-1) + (n - 1) = n^3 - 1^3
$$

We can cancel -1 on both sides:
$$
3[1^2 + 2^2 + ... + (n - 1)^2] + \frac{3}{2}n(n-1) + n = n^3
$$

Moving the terms to the right:
$$
3[1^2 + 2^2 + ... + (n - 1)^2] = n^3 - \frac{3}{2}n^2 + \frac{3}{2}n - n
$$

Finally:
$$
1^2 + 2^2 + ... + (n - 1)^2 = \frac{n^3}{3} - \frac{n^2}{2} + \frac{n}{6}
$$

Adding $n$ on both sides:
$$
1^2 + 2^2 + ... + n^2 = \frac{n^3}{3} + \frac{n^2}{2} + \frac{n}{6}
$$

\end{document}
